src/program_proof/tulip/program/txn/txn.v
@@ -1,0 +1,1917 @@
+From Perennial.program_proof.tulip.invariance Require Import
+  read commit abort cancel linearize preprepare unprepare prepare.
+From Perennial.program_proof.tulip.program Require Import prelude.
+From Perennial.program_proof.tulip.program Require Import prelude group_coordinator.
+From Perennial.goose_lang.trusted.github_com.mit_pdos.tulip Require Import trusted_proph.
+
+Section res.
+  Context `{!heapGS Σ}.
+
+  Definition txnmap_auth (τ : gname) (m : dbmap) : iProp Σ.
+  Admitted.
+
+  Definition txnmap_ptsto (τ : gname) (k : dbkey) (v : dbval) : iProp Σ.
+  Admitted.
+
+  Definition txnmap_ptstos (τ : gname) (m : dbmap) : iProp Σ :=
+    [∗ map] k ↦ v ∈ m, txnmap_ptsto τ k v.
+
+  Lemma txnmap_alloc m :
+    ⊢ |==> ∃ τ, txnmap_auth τ m ∗ ([∗ map] k ↦ v ∈ m, txnmap_ptsto τ k v).
+  Admitted.
+
+  Lemma txnmap_lookup τ m k v :
+    txnmap_auth τ m -∗
+    txnmap_ptsto τ k v -∗
+    ⌜m !! k = Some v⌝.
+  Admitted.
+
+  Lemma txnmap_update {τ m k v1} v2 :
+    txnmap_auth τ m -∗
+    txnmap_ptsto τ k v1 ==∗
+    txnmap_auth τ (<[k := v2]> m) ∗ txnmap_ptsto τ k v2.
+  Admitted.
+
+  Lemma txnmap_subseteq τ m1 m2 :
+    txnmap_auth τ m1 -∗
+    txnmap_ptstos τ m2 -∗
+    ⌜m2 ⊆ m1⌝.
+  Admitted.
+
+  Definition local_gid_token (α : gname) (gid : u64) : iProp Σ.
+  Admitted.
+
+  Lemma local_gid_tokens_alloc (gids : gset u64) :
+    ⊢ |==> ∃ α, [∗ set] gid ∈ gids, local_gid_token α gid.
+  Admitted.
+
+  Lemma local_gid_token_ne (α : gname) (gid1 gid2 : u64) :
+    local_gid_token α gid1 -∗
+    local_gid_token α gid2 -∗
+    ⌜gid2 ≠ gid1⌝.
+  Admitted.
+
+End res.
+
+Section repr.
+  Context `{!heapGS Σ, !tulip_ghostG Σ}.
+
+  (*@ type Txn struct {                                                       @*)
+  (*@     // Timestamp of this transaction.                                   @*)
+  (*@     ts      uint64                                                      @*)
+  (*@     // Buffered write set.                                              @*)
+  (*@     wrs     map[uint64]map[string]tulip.Value                           @*)
+  (*@     // Participant group of this transaction. Initialized in prepare time. @*)
+  (*@     ptgs    []uint64                                                    @*)
+  (*@     // Group coordinators for performing reads, prepare, abort, and commit. @*)
+  (*@     gcoords map[uint64]*gcoord.GroupCoordinator                         @*)
+  (*@     // Global prophecy variable (for verification purpose).             @*)
+  (*@     proph   primitive.ProphId                                           @*)
+  (*@ }                                                                       @*)
+  Definition txn_wrs (wrsP : loc) q (wrs : dbmap) : iProp Σ :=
+    ∃ (pwrsmP : gmap u64 loc) (pwrsm : gmap u64 dbmap),
+      "HpwrsmP"  ∷ own_map wrsP (DfracOwn 1) pwrsmP ∗
+      "Hpwrsm"   ∷ ([∗ map] p; m ∈ pwrsmP; pwrsm, own_map p q m) ∗
+      "%Hwrsg"   ∷ ⌜map_Forall (λ g m, m = wrs_group g wrs) pwrsm⌝ ∗
+      "%Hdomwrs" ∷ ⌜dom pwrsmP = gids_all⌝.
+
+  Definition own_txn_wrs txn q (wrs : dbmap) : iProp Σ :=
+    ∃ (wrsP : loc) (wrspP : loc),
+      "HwrsP"  ∷ txn ↦[Txn :: "wrs"] #wrsP ∗
+      "Hwrs"   ∷ txn_wrs wrsP q wrs ∗
+      "HwrspP" ∷ txn ↦[Txn :: "wrsp"] #wrspP ∗
+      "Hwrsp"  ∷ own_map wrspP (DfracOwn 1) wrs.
+
+  Definition own_txn_ptgs txn (ptgs : list u64) : iProp Σ :=
+    ∃ (ptgsS : Slice.t),
+      "HptgsS" ∷ txn ↦[Txn :: "ptgs"] (to_val ptgsS) ∗
+      "Hptgs"  ∷ own_slice ptgsS uint64T (DfracOwn 1) ptgs ∗
+      "%Hnd"   ∷ ⌜NoDup ptgs⌝.
+
+  Definition own_txn_ts txn (tid : nat) : iProp Σ :=
+    ∃ (tsW : u64),
+      "HtsW"     ∷ txn ↦[Txn :: "ts"] #tsW ∗
+      "%Htsword" ∷ ⌜uint.nat tsW = tid⌝.
+
+  Definition own_txn_gcoords txn γ : iProp Σ :=
+    ∃ (gcoordsP : loc) (gcoords : gmap u64 loc),
+      "HgcoordsP"    ∷ txn ↦[Txn :: "gcoords"] #gcoordsP ∗
+      "Hgcoords"     ∷ own_map gcoordsP (DfracOwn 1) gcoords ∗
+      "#Hgcoordsabs" ∷ ([∗ map] gid ↦ gcoord ∈ gcoords, is_gcoord gcoord gid γ) ∗
+      "%Hdomgcoords" ∷ ⌜dom gcoords = gids_all⌝.
+
+  Definition own_txn_internal txn tid γ : iProp Σ :=
+    ∃ (proph : proph_id),
+      "Hts"      ∷ own_txn_ts txn tid ∗
+      "Hwrs"     ∷ own_txn_wrs txn (DfracOwn 1) ∅ ∗
+      "Hgcoords" ∷ own_txn_gcoords txn γ ∗
+      "Hptgs"    ∷ own_txn_ptgs txn [] ∗
+      "HprophP"  ∷ txn ↦[Txn :: "proph"] #proph ∗
+      "#Hinv"    ∷ know_tulip_inv_with_proph γ proph.
+
+  Definition own_txn_uninit txn γ : iProp Σ :=
+    ∃ tid, "Htxn" ∷ own_txn_internal txn tid γ.
+
+  Definition own_txn_init txn tid γ : iProp Σ :=
+    "Htxn"  ∷ own_txn_internal txn tid γ ∗
+    "%Hvts" ∷ ⌜valid_ts tid⌝.
+
+  Definition own_txn txn tid rds γ τ : iProp Σ :=
+    ∃ (proph : proph_id) wrs,
+      "Htxn"     ∷ own_txn_ts txn tid ∗
+      "Hwrs"     ∷ own_txn_wrs txn (DfracOwn 1) wrs ∗
+      "Hgcoords" ∷ own_txn_gcoords txn γ ∗
+      "Hptgs"    ∷ own_txn_ptgs txn [] ∗
+      (* diff from [own_txn_init] *)
+      "Htxnmap"  ∷ txnmap_auth τ (wrs ∪ rds) ∗
+      "HprophP"  ∷ txn ↦[Txn :: "proph"] #proph ∗
+      "#Hinv"    ∷ know_tulip_inv_with_proph γ proph ∗
+      (* diff from [own_txn_init] *)
+      "#Hlnrz"   ∷ ([∗ map] key ↦ value ∈ rds, is_lnrz_hist_at γ key (pred tid) value) ∗
+      "%Hdomr"   ∷ ⌜dom rds ⊆ keys_all⌝ ∗
+      (* diff from [own_txn_init] *)
+      "%Hincl"   ∷ ⌜dom wrs ⊆ dom rds⌝ ∗
+      "%Hvts"    ∷ ⌜valid_ts tid⌝ ∗
+      (* diff from [own_txn_init] *)
+      "%Hvwrs"   ∷ ⌜valid_wrs wrs⌝.
+
+    Definition own_txn_stable txn tid rds wrs γ τ : iProp Σ :=
+    ∃ (proph : proph_id),
+      "Htxn"     ∷ own_txn_ts txn tid ∗
+      (* diff from [own_txn] *)
+      "Hwrs"     ∷ own_txn_wrs txn DfracDiscarded wrs ∗
+      "Hgcoords" ∷ own_txn_gcoords txn γ ∗
+      "Hptgs"    ∷ own_txn_ptgs txn [] ∗
+      "Htxnmap"  ∷ txnmap_auth τ (wrs ∪ rds) ∗
+      "HprophP"  ∷ txn ↦[Txn :: "proph"] #proph ∗
+      "#Hinv"    ∷ know_tulip_inv_with_proph γ proph ∗
+      "#Hlnrz"   ∷ ([∗ map] key ↦ value ∈ rds, is_lnrz_hist_at γ key (pred tid) value) ∗
+      "%Hdomr"   ∷ ⌜dom rds ⊆ keys_all⌝ ∗
+      (* diff from [own_txn] and [wrs] is exposed *)
+      "#Htxnwrs" ∷ is_txn_wrs γ tid wrs ∗
+      "%Hincl"   ∷ ⌜dom wrs ⊆ dom rds⌝ ∗
+      "%Hvts"    ∷ ⌜valid_ts tid⌝ ∗
+      "%Hvwrs"   ∷ ⌜valid_wrs wrs⌝.
+
+  Definition own_txn_prepared txn tid rds wrs γ τ : iProp Σ :=
+    ∃ (proph : proph_id) ptgs,
+      "Htxn"     ∷ own_txn_ts txn tid ∗
+      "Hwrs"     ∷ own_txn_wrs txn DfracDiscarded wrs ∗
+      "Hgcoords" ∷ own_txn_gcoords txn γ ∗
+      (* diff from [own_txn_stable] *)
+      "Hptgs"    ∷ own_txn_ptgs txn ptgs ∗
+      "Htxnmap"  ∷ txnmap_auth τ (wrs ∪ rds) ∗
+      "HprophP"  ∷ txn ↦[Txn :: "proph"] #proph ∗
+      "#Hinv"    ∷ know_tulip_inv_with_proph γ proph ∗
+      "#Hlnrz"   ∷ ([∗ map] key ↦ value ∈ rds, is_lnrz_hist_at γ key (pred tid) value) ∗
+      "#Htxnwrs" ∷ is_txn_wrs γ tid wrs ∗
+      "%Hdomr"   ∷ ⌜dom rds ⊆ keys_all⌝ ∗
+      "%Hincl"   ∷ ⌜dom wrs ⊆ dom rds⌝ ∗
+      "%Hvts"    ∷ ⌜valid_ts tid⌝ ∗
+      "%Hvwrs"   ∷ ⌜valid_wrs wrs⌝ ∗
+      (* diff from [own_txn_stable] *)
+      "%Hptgs"   ∷ ⌜list_to_set ptgs = ptgroups (dom wrs)⌝.
+
+End repr.
+
+Section proph.
+  Context `{!heapGS Σ, !tulip_ghostG Σ}.
+
+  Lemma wp_ResolveRead p (tid : u64) (key : string) (ts : nat) :
+    ⊢
+    {{{ ⌜uint.nat tid = ts⌝ }}}
+    <<< ∀∀ acs, own_txn_proph p acs >>>
+      ResolveRead #p #tid #(LitString key) @ ∅
+    <<< ∃ acs', ⌜acs = ActRead ts key :: acs'⌝ ∗ own_txn_proph p acs' >>>
+    {{{ RET #(); True }}}.
+  Admitted.
+
+  Lemma wp_ResolveAbort p (tid : u64) (ts : nat) :
+    ⊢
+    {{{ ⌜uint.nat tid = ts⌝ }}}
+    <<< ∀∀ acs, own_txn_proph p acs >>>
+      ResolveAbort #p #tid @ ∅
+    <<< ∃ acs', ⌜acs = ActAbort ts :: acs'⌝ ∗ own_txn_proph p acs' >>>
+    {{{ RET #(); True }}}.
+  Admitted.
+
+  Lemma wp_ResolveCommit
+    p (tid : u64) (ts : nat) (wrsP : loc) q (wrs : dbmap) :
+    ⊢
+    {{{ ⌜uint.nat tid = ts⌝ ∗ own_map wrsP q wrs }}}
+    <<< ∀∀ acs, own_txn_proph p acs >>>
+      ResolveCommit #p #tid #wrsP @ ∅
+    <<< ∃ acs', ⌜acs = ActCommit ts wrs :: acs'⌝ ∗ own_txn_proph p acs' >>>
+    {{{ RET #(); own_map wrsP q wrs }}}.
+  Admitted.
+
+End proph.
+
+Section program.
+  Context `{!heapGS Σ, !tulip_ghostG Σ}.
+
+  Theorem wp_KeyToGroup (key : string) :
+    {{{ True }}}
+      KeyToGroup #(LitString key)
+    {{{ (gid : u64), RET #gid; ⌜key_to_group key = gid⌝ }}}.
+  Proof.
+    (*@ func KeyToGroup(key string) uint64 {                                    @*)
+    (*@     // TODO                                                             @*)
+    (*@     return 0                                                            @*)
+    (*@ }                                                                       @*)
+  Admitted.
+
+    Theorem wp_Txn__getwrs (txn : loc) (key : string) q wrs :
+    {{{ own_txn_wrs txn q wrs }}}
+      Txn__getwrs #txn #(LitString key)
+    {{{ (v : dbval) (ok : bool), RET (dbval_to_val v, #ok);
+        own_txn_wrs txn q wrs ∗ ⌜wrs !! key = if ok then Some v else None⌝
+    }}}.
+  Proof.
+    iIntros (Φ) "Hwrs HΦ".
+    wp_rec.
+
+    (*@ func (txn *Txn) getwrs(key string) (Value, bool) {                      @*)
+    (*@     gid := KeyToGroup(key)                                              @*)
+    (*@     pwrs := txn.wrs[gid]                                                @*)
+    (*@                                                                         @*)
+    wp_apply wp_KeyToGroup.
+    iIntros (gid Hgid).
+    do 2 iNamed "Hwrs".
+    wp_loadField.
+    wp_apply (wp_MapGet with "HpwrsmP").
+    iIntros (pwrsP ok) "[%Hget HpwrsmP]".
+    destruct ok; last first.
+    { apply map_get_false in Hget as [Hget _].
+      rewrite -not_elem_of_dom Hdomwrs -Hgid in Hget.
+      by pose proof (elem_of_key_to_group key).
+    }
+    apply map_get_true in Hget.
+    iAssert (⌜is_Some (pwrsm !! gid)⌝)%I as %[pwrs Hpwrs].
+    { iDestruct (big_sepM2_dom with "Hpwrsm") as %Hdom.
+      iPureIntro.
+      by rewrite -elem_of_dom -Hdom elem_of_dom.
+    }
+    iDestruct (big_sepM2_lookup_acc with "Hpwrsm") as "[Hpwrs HpwrsmC]"; [done | done |].
+
+    (*@     v, ok := pwrs[key]                                                  @*)
+    (*@     return v, ok                                                        @*)
+    (*@ }                                                                       @*)
+    wp_apply (wp_MapGet with "Hpwrs").
+    iIntros (v ok) "[%Hv Hpwrs]".
+    wp_pures.
+    iApply "HΦ".
+    iDestruct ("HpwrsmC" with "Hpwrs") as "Hpwrsm".
+    iFrame "∗ # %".
+    iPureIntro.
+    specialize (Hwrsg _ _ Hpwrs). simpl in Hwrsg.
+    rewrite Hwrsg in Hv.
+    destruct ok.
+    - apply map_get_true in Hv.
+      rewrite lookup_wrs_group_Some in Hv.
+      by destruct Hv as [Hv _].
+    - apply map_get_false in Hv as [Hv _].
+      rewrite lookup_wrs_group_None in Hv.
+      by destruct Hv.
+  Qed.
+
+  Theorem wp_Txn__setwrs (txn : loc) (key : string) (value : dbval) wrs :
+    {{{ own_txn_wrs txn (DfracOwn 1) wrs }}}
+      Txn__setwrs #txn #(LitString key) (dbval_to_val value)
+    {{{ RET #(); own_txn_wrs txn (DfracOwn 1) (<[key := value]> wrs) }}}.
+  Proof.
+    iIntros (Φ) "Hwrs HΦ".
+    wp_rec.
+
+    (*@ func (txn *Txn) setwrs(key string, value Value) {                       @*)
+    (*@     gid := KeyToGroup(key)                                              @*)
+    (*@     pwrs := txn.wrs[gid]                                                @*)
+    (*@                                                                         @*)
+    wp_apply wp_KeyToGroup.
+    iIntros (gid Hgid).
+    do 2 iNamed "Hwrs".
+    wp_loadField.
+    wp_apply (wp_MapGet with "HpwrsmP").
+    iIntros (pwrsP ok) "[%Hget HpwrsmP]".
+    destruct ok; last first.
+    { apply map_get_false in Hget as [Hget _].
+      rewrite -not_elem_of_dom Hdomwrs -Hgid in Hget.
+      by pose proof (elem_of_key_to_group key).
+    }
+    apply map_get_true in Hget.
+    iAssert (⌜is_Some (pwrsm !! gid)⌝)%I as %[pwrs Hpwrs].
+    { iDestruct (big_sepM2_dom with "Hpwrsm") as %Hdom.
+      iPureIntro.
+      by rewrite -elem_of_dom -Hdom elem_of_dom.
+    }
+    iDestruct (big_sepM2_delete with "Hpwrsm") as "[Hpwrs Hpwrsm]"; [done | done |].
+
+    (*@     pwrs[key] = value                                                   @*)
+    (*@ }                                                                       @*)
+    wp_apply (wp_MapInsert with "Hpwrs"); first done.
+    iIntros "Hpwrs".
+    wp_loadField.
+    wp_apply (wp_MapInsert with "Hwrsp"); first done.
+    iIntros "Hwrsp".
+    wp_pures.
+    iApply "HΦ".
+    set pwrs' := <[key := value]> pwrs.
+    iAssert ([∗ map] p; m ∈ pwrsmP; <[gid := pwrs']> pwrsm, own_map p (DfracOwn 1) m)%I
+      with "[Hpwrsm Hpwrs]" as "Hpwrsm".
+    { iDestruct (big_sepM2_insert_2 (λ k p m, own_map p (DfracOwn 1) m) _ _ gid with "Hpwrs Hpwrsm")
+        as "Hpwrsm".
+      rewrite insert_delete; last apply Hget.
+      rewrite insert_delete_insert.
+      done.
+    }
+    iFrame "∗ %".
+    iPureIntro.
+    intros g m Hgm.
+    destruct (decide (gid = g)) as [-> | Hne].
+    - rewrite lookup_insert in Hgm. inv Hgm.
+      specialize (Hwrsg _ _ Hpwrs). simpl in Hwrsg.
+      by rewrite Hwrsg wrs_group_insert.
+    - rewrite lookup_insert_ne in Hgm; last done.
+      specialize (Hwrsg _ _ Hgm). simpl in Hwrsg.
+      subst m.
+      by rewrite wrs_group_insert_ne; last rewrite Hgid.
+  Qed.
+
+  Theorem wp_Txn__resetwrs (txn : loc) q wrs :
+    {{{ own_txn_wrs txn q wrs }}}
+      Txn__resetwrs #txn
+    {{{ RET #(); own_txn_wrs txn (DfracOwn 1) ∅ }}}.
+  Proof.
+    iIntros (Φ) "Hwrs HΦ".
+    wp_rec.
+
+    (*@ func (txn *Txn) resetwrs() {                                            @*)
+    (*@     // Creating a new @wrs is not really necessary, but currently it seems like @*)
+    (*@     // there's no easy way to reason modifying a map while iterating over it @*)
+    (*@     // (which is a defined behavior in Go).                             @*)
+    (*@     wrs := make(map[uint64]map[string]tulip.Value)                      @*)
+    (*@     for gid := range(txn.wrs) {                                         @*)
+    (*@         wrs[gid] = make(map[string]tulip.Value)                         @*)
+    (*@     }                                                                   @*)
+    (*@     txn.wrs = wrs                                                       @*)
+    (*@     txn.wrsp = make(map[string]tulip.Value)                             @*)
+    (*@ }                                                                       @*)
+    wp_apply wp_NewMap.
+    iIntros (wrsP') "HpwrsmP'".
+    do 2 iNamed "Hwrs".
+    (* iDestruct (big_sepM2_dom with "Hpwrsm") as %Hdom. *)
+    wp_loadField.
+    set P := (λ (mx : gmap u64 loc),
+      let em := gset_to_gmap (∅ : dbmap) (dom mx) in
+      ∃ (pwrsmP' : gmap u64 loc),
+        "HpwrsmP'" ∷ own_map wrsP' (DfracOwn 1) pwrsmP' ∗
+        "Hpwrsm'"  ∷ ([∗ map] p;m ∈ pwrsmP';em, own_map p (DfracOwn 1) m))%I.
+    wp_apply (wp_MapIter_fold _ _ _ P with "HpwrsmP [HpwrsmP']").
+    { subst P. simpl.
+      rewrite dom_empty_L gset_to_gmap_empty.
+      iFrame.
+      by iApply big_sepM2_empty.
+    }
+    { clear Φ.
+      iIntros (m gid pwrsP Φ) "!> [HP [%Hnone %Hsome]] HΦ".
+      iNamed "HP".
+      wp_pures.
+      wp_apply wp_NewMap.
+      iIntros (empP) "HempP".
+      wp_apply (wp_MapInsert with "HpwrsmP'"); first by auto.
+      iIntros "HpwrsmP'".
+      iApply "HΦ".
+      subst P. simpl.
+      iFrame.
+      rewrite dom_insert_L gset_to_gmap_union_singleton.
+      iApply (big_sepM2_insert_2 with "[HempP] Hpwrsm'"); first iFrame.
+    }
+    iIntros "[HpwrsmP HP]".
+    subst P. simpl.
+    iNamed "HP".
+    wp_storeField.
+    wp_apply wp_NewMap.
+    iIntros (wrspP') "HwrspP'".
+    wp_storeField.
+    iApply "HΦ".
+    iDestruct (big_sepM2_dom with "Hpwrsm'") as %Hdom'.
+    iFrame "∗ %".
+    iPureIntro.
+    split; last first.
+    { by rewrite Hdom' dom_gset_to_gmap Hdomwrs. }
+    intros g m Hgm.
+    rewrite lookup_gset_to_gmap_Some in Hgm.
+    destruct Hgm as [_ Hm].
+    by rewrite /wrs_group map_filter_empty.
+  Qed.
+
+  Theorem wp_Txn__setptgs txn q wrs :
+    {{{ own_txn_wrs txn q wrs ∗ own_txn_ptgs txn [] }}}
+      Txn__setptgs #txn
+    {{{ RET #(); ∃ ptgs, own_txn_wrs txn q wrs ∗ own_txn_ptgs txn ptgs ∗
+                         ⌜list_to_set ptgs = ptgroups (dom wrs)⌝
+    }}}.
+  Proof using heapGS0 tulip_ghostG0 Σ.
+    iIntros (Φ) "[Hwrs Hptgs] HΦ".
+    wp_rec.
+
+    (*@ func (txn *Txn) setptgs() {                                             @*)
+    (*@     var ptgs = txn.ptgs                                                 @*)
+    (*@                                                                         @*)
+    iNamed "Hptgs".
+    clear Hnd.
+    wp_loadField.
+    wp_apply wp_ref_to; first apply slice_val_ty.
+    iIntros (ptgsP) "HptgsP".
+
+    (*@     for gid, pwrs := range(txn.wrs) {                                   @*)
+    (*@         if uint64(len(pwrs)) != 0 {                                     @*)
+    (*@             ptgs = append(ptgs, gid)                                    @*)
+    (*@         }                                                               @*)
+    (*@     }                                                                   @*)
+    (*@     txn.ptgs = ptgs                                                     @*)
+    (*@ }                                                                       @*)
+    do 2 iNamed "Hwrs".
+    wp_loadField.
+    set P := (λ (mx : gmap u64 loc),
+      ∃ (s : Slice.t) (ptgs : list u64),
+        "HptgsP" ∷ ptgsP ↦[slice.T uint64T] (to_val s) ∗
+        "Hptgs"  ∷ own_slice s uint64T (DfracOwn 1) ptgs ∗
+        "Hpwrsm" ∷ ([∗ map] p;m ∈ pwrsmP;pwrsm, own_map p q m) ∗
+        "%Hnd"   ∷ ⌜NoDup ptgs⌝ ∗
+        "%Hincl" ∷ ⌜Forall (λ g, g ∈ dom mx) ptgs⌝ ∗
+        (* non-empty ↔ in ptgs *)
+        "%Hspec" ∷ ⌜set_Forall (λ g, keys_group g (dom wrs) ≠ ∅ ↔ g ∈ ptgs) (dom mx)⌝)%I.
+    wp_apply (wp_MapIter_fold _ _ _ P with "HpwrsmP [$HptgsP $Hptgs $Hpwrsm]").
+    { iPureIntro. by split; first apply NoDup_nil. }
+    { clear Φ.
+      iIntros (m gid pwrsP Φ) "!> [HP [%Hnone %Hsome]] HΦ".
+      iNamed "HP".
+      iAssert (⌜is_Some (pwrsm !! gid)⌝)%I as %[pwrs Hpwrs].
+      { iDestruct (big_sepM2_dom with "Hpwrsm") as %Hdom.
+        iPureIntro.
+        by rewrite -elem_of_dom -Hdom elem_of_dom.
+      }
+      iDestruct (big_sepM2_lookup_acc with "Hpwrsm") as "[Hpwrs HpwrsmC]"; [done | done |].
+      wp_apply (wp_MapLen with "Hpwrs").
+      iIntros "[%Hsize Hpwrs]".
+      iDestruct ("HpwrsmC" with "Hpwrs") as "Hpwrsm".
+      wp_if_destruct.
+      { wp_load.
+        (* NB: need to provide [own_slice] to properly resolve the right typeclass. *)
+        wp_apply (wp_SliceAppend with "Hptgs").
+        iIntros (s') "Hptgs".
+        wp_store.
+        iApply "HΦ".
+        iFrame.
+        iPureIntro.
+        split.
+        { apply NoDup_snoc; last apply Hnd.
+          intros Hgid.
+          rewrite Forall_forall in Hincl.
+          specialize (Hincl _ Hgid).
+          by apply not_elem_of_dom in Hnone.
+        }
+        split.
+        { rewrite Forall_app Forall_singleton dom_insert_L.
+          split; last set_solver.
+          apply (Forall_impl _ _ _ Hincl).
+          set_solver.
+        }
+        intros g Hg.
+        rewrite dom_insert_L elem_of_union in Hg.
+        split.
+        { intros Hne.
+          destruct Hg as [? | Hg]; first set_solver.
+          specialize (Hspec _ Hg). simpl in Hspec.
+          set_solver.
+        }
+        { intros Hsnoc.
+          destruct Hg as [Hgid | Hg]; last first.
+          { specialize (Hspec _ Hg). simpl in Hspec.
+            apply Hspec.
+            rewrite -not_elem_of_dom in Hnone.
+            set_solver.
+          }
+          rewrite elem_of_singleton in Hgid.
+          subst g.
+          (* FIXME: not sure if word is supposed to solve this immediately *)
+          assert (Hnz : size pwrs ≠ O).
+          { intros Hz. rewrite Hz in Heqb. word. }
+          clear Heqb.
+          specialize (Hwrsg _ _ Hpwrs). simpl in Hwrsg.
+          intros Hempty.
+          rewrite -wrs_group_keys_group_dom -Hwrsg in Hempty.
+          apply dom_empty_inv_L in Hempty.
+          by rewrite map_size_non_empty_iff in Hnz.
+        }
+      }
+      iApply "HΦ".
+      iFrame.
+      iPureIntro.
+      rewrite dom_insert_L.
+      split; first apply Hnd.
+      split.
+      { apply (Forall_impl _ _ _ Hincl). set_solver. }
+      apply set_Forall_union; last apply Hspec.
+      rewrite set_Forall_singleton.
+      assert (Hsizez : size pwrs = O).
+      { rewrite Heqb in Hsize. done. }
+      split.
+      { intros Hne.
+        specialize (Hwrsg _ _ Hpwrs). simpl in Hwrsg.
+        rewrite -wrs_group_keys_group_dom -Hwrsg in Hne.
+        apply map_size_empty_inv in Hsizez.
+        by rewrite Hsizez in Hne.
+      }
+      { intros Hinptgs.
+        rewrite Forall_forall in Hincl.
+        specialize (Hincl _ Hinptgs).
+        by rewrite -not_elem_of_dom in Hnone.
+      }
+    }
+    iIntros "[HpwrsmP HP]". 
+    iNamed "HP".
+    wp_load. wp_storeField.
+    iApply "HΦ".
+    iFrame "∗ # %".
+    iPureIntro.
+    apply set_eq.
+    intros gid.
+    rewrite elem_of_ptgroups elem_of_list_to_set.
+    split.
+    { intros Hgid.
+      rewrite Forall_forall in Hincl.
+      specialize (Hincl _ Hgid).
+      specialize (Hspec _ Hincl). simpl in Hspec.
+      by apply Hspec.
+    }
+    { intros Hne.
+      destruct (decide (gid ∈ gids_all)) as [Hin | Hnotin]; last first.
+      { rewrite /keys_group in Hne.
+        apply set_choose_L in Hne as [k Hk].
+        pose proof (elem_of_key_to_group k) as Hin.
+        set_solver.
+      }
+      rewrite Hdomwrs in Hspec.
+      specialize (Hspec _ Hin). simpl in Hspec.
+      by apply Hspec.
+    }
+  Qed.
+
+  Theorem wp_Txn__resetptgs (txn : loc) ptgs :
+    {{{ own_txn_ptgs txn ptgs }}}
+      Txn__resetptgs #txn
+    {{{ RET #(); own_txn_ptgs txn [] }}}.
+  Proof.
+    iIntros (Φ) "Hptgs HΦ".
+    wp_rec.
+
+    (*@ func (txn *Txn) resetptgs() {                                           @*)
+    (*@     txn.ptgs = txn.ptgs[:0]                                             @*)
+    (*@ }                                                                       @*)
+    iNamed "Hptgs".
+    wp_loadField.
+    wp_apply wp_SliceTake; first word.
+    wp_storeField.
+    iApply "HΦ".
+    iDestruct (own_slice_take_cap _ _ _ (W64 0) with "Hptgs") as "Hptgs"; first word.
+    iFrame.
+    iPureIntro.
+    by apply NoDup_nil.
+  Qed.
+
+  Theorem wp_Txn__reset (txn : loc) wrs q ptgs :
+    {{{ own_txn_wrs txn q wrs ∗ own_txn_ptgs txn ptgs }}}
+      Txn__reset #txn
+    {{{ RET #(); own_txn_wrs txn (DfracOwn 1) ∅ ∗ own_txn_ptgs txn [] }}}.
+  Proof.
+    iIntros (Φ) "[Hwrs Hptgs] HΦ".
+    wp_rec.
+
+    (*@ func (txn *Txn) reset() {                                               @*)
+    (*@     txn.resetwrs()                                                      @*)
+    (*@     txn.resetptgs()                                                     @*)
+    (*@ }                                                                       @*)
+    wp_apply (wp_Txn__resetwrs with "Hwrs").
+    iIntros "Hwrs".
+    wp_apply (wp_Txn__resetptgs with "Hptgs").
+    iIntros "Hptgs".
+    wp_pures.
+    iApply "HΦ".
+    by iFrame.
+  Qed.
+
+  Theorem wp_Txn__commit txn tid rds wrsphys wrsproph γ τ :
+    is_lnrz_tid γ tid -∗
+    all_prepared γ tid wrsphys -∗
+    {{{ own_txn_prepared txn tid rds wrsphys γ τ ∗ own_cmt_tmod γ tid wrsproph }}}
+      Txn__commit #txn
+    {{{ RET #(); own_txn_uninit txn γ ∗ ⌜wrsphys = wrsproph⌝ }}}.
+  Proof.
+    iIntros "#Hlnrzed #Hprep" (Φ) "!> [Htxn Htidc] HΦ".
+    wp_rec.
+
+    (*@ func (txn *Txn) commit() {                                              @*)
+    (*@     ResolveCommit(txn.proph, txn.ts, txn.wrs)                           @*)
+    (*@                                                                         @*)
+    do 2 iNamed "Htxn". iNamed "Hwrs".
+    do 3 wp_loadField.
+    wp_apply (wp_ResolveCommit with "[$Hwrsp]"); first done.
+    iInv "Hinv" as "> HinvO" "HinvC".
+    iApply ncfupd_mask_intro; first set_solver.
+    iIntros "Hmask".
+    iNamed "HinvO".
+    iDestruct (txnsys_inv_extract_future with "Htxnsys") as (future) "[Hproph Htxnsys]".
+    iFrame "Hproph".
+    iIntros "(%future' & %Hfuture & Hproph)".
+    iMod (txnsys_inv_commit with "Hlnrzed Hprep Htxnsys Hgroups Hrgs Hkeys")
+      as "(Htxnsys & Hgroups & Hrgs & Hkeys & #Hcmt)".
+    { by rewrite Hfuture. }
+    iAssert (⌜wrsphys = wrsproph⌝)%I as %Heq.
+    { do 2 iNamed "Htxnsys".
+      iDestruct (txn_res_lookup with "Hresm Hcmt") as %Hwrsc.
+      iDestruct (elem_of_committed_partitioned_tids with "Hpart") as %[Hnotinwc Hnotinwa].
+      { by eauto. }
+      iDestruct (cmt_tmod_lookup with "Htidcs Htidc") as %Htidc.
+      specialize (Htidcs _ _ Htidc). simpl in Htidcs.
+      (* Prove [resm !! tid = Some (ResCommitted wrs)]. *)
+      destruct Htidcs as [Htmodcs | Hresm].
+      { by rewrite not_elem_of_dom Htmodcs in Hnotinwc. }
+      rewrite Hresm in Hwrsc. symmetry in Hwrsc. inv Hwrsc.
+      done.
+    }
+    (* Close the invariant. *)
+    rewrite Hfuture /=.
+    iDestruct (txnsys_inv_merge_future with "Hproph Htxnsys") as "Htxnsys".
+    iMod "Hmask" as "_".
+    iMod ("HinvC" with "[Htxnsys Hkeys Hgroups Hrgs]") as "_"; first by iFrame.
+    iIntros "!> Hwrsp".
+    wp_pures.
+    do 2 wp_loadField.
+
+    (*@     ts := txn.ts                                                        @*)
+    (*@     for _, gid := range(txn.ptgs) {                                     @*)
+    (*@                                                                         @*)
+    iNamed "Hptgs". iNamed "Hwrs".
+    iDestruct "Hpwrsm" as "#Hpwrsm".
+    wp_loadField.
+    set P := (λ (_ : u64),
+                "HpwrsmP" ∷ own_map wrsP (DfracOwn 1) pwrsmP ∗
+                "Hgcoords" ∷ own_txn_gcoords txn γ)%I.
+    iDestruct (own_slice_small_acc with "Hptgs") as "[Hptgs HptgsC]".
+    wp_apply (wp_forSlice P with "[] [$Hptgs $HpwrsmP $Hgcoords]").
+    { (* Loop body. *)
+      clear Φ.
+
+      (*@         gcoord := txn.gcoords[gid]                                      @*)
+      (*@         pwrs := txn.wrs[gid]                                            @*)
+      (*@                                                                         @*)
+      iIntros (i gid Φ) "!> (HP & %Hinbound & %Hgid) HΦ".
+      iNamed "HP". iNamed "Hgcoords".
+      wp_loadField.
+      assert (Hin : gid ∈ gids_all).
+      { pose proof (subseteq_ptgroups (dom wrsphys)) as Hdom.
+        apply elem_of_list_lookup_2 in Hgid.
+        clear -Hdom Hgid Hptgs.
+        set_solver.
+      }
+      wp_apply (wp_MapGet with "Hgcoords").
+      iIntros (gcoordP ok) "[%Hgetgcoords Hgcoords]".
+      destruct ok; last first.
+      { apply map_get_false in Hgetgcoords as [Hnone _].
+        by rewrite -not_elem_of_dom Hdomgcoords in Hnone.
+      }
+      apply map_get_true in Hgetgcoords.
+      wp_apply (wp_MapGet with "HpwrsmP").
+      iIntros (pwrsP ok) "[%Hgetwrs HpwrsmP]".
+      destruct ok; last first.
+      { apply map_get_false in Hgetwrs as [Hnotin _].
+        by rewrite -not_elem_of_dom Hdomwrs in Hnotin.
+      }
+      apply map_get_true in Hgetwrs.
+      iAssert (⌜is_Some (pwrsm !! gid)⌝)%I as %[pwrs Hpwrs].
+      { iDestruct (big_sepM2_dom with "Hpwrsm") as %Hdom.
+        iPureIntro.
+        by rewrite -elem_of_dom -Hdom elem_of_dom.
+      }
+      iDestruct (big_sepM2_lookup_acc with "Hpwrsm") as "[Hpwrs HpwrsmC]"; [done | done |].
+
+      (*@         go func() {                                                     @*)
+      (*@             gcoord.Commit(ts, pwrs)                                     @*)
+      (*@         }()                                                             @*)
+      (*@     }                                                                   @*)
+      (*@                                                                         @*)
+      wp_pures.
+      iDestruct (big_sepM_lookup with "Hgcoordsabs") as "Hgcoordabs"; first apply Hgetgcoords.
+      wp_apply wp_fork.
+      { wp_apply (wp_GroupCoordinator__Commit with "[] Hgcoordabs Hpwrs").
+        { rewrite Htsword.
+          iFrame "Hcmt Htxnwrs".
+          iPureIntro.
+          assert (Hinptgs : gid ∈ ptgroups (dom wrsphys)).
+          { rewrite -Hptgs elem_of_list_to_set elem_of_list_lookup. by eauto. }
+          specialize (Hwrsg _ _ Hpwrs).
+          done.
+        }
+        by iIntros "_".
+      }
+      iApply "HΦ".
+      iFrame "∗ # %".
+    }
+    iIntros "[HP Hptgs]".
+    iNamed "HP". clear P.
+    iDestruct ("HptgsC" with "Hptgs") as "Hptgs".
+    iAssert (own_txn_ptgs txn ptgs)%I with "[$HptgsS $Hptgs]" as "Hptgs"; first done.
+
+    (*@     txn.reset()                                                         @*)
+    (*@ }                                                                       @*)
+    iAssert (own_txn_wrs txn DfracDiscarded wrsphys)%I
+      with "[$HwrsP $HwrspP $Hwrsp $HpwrsmP]" as "Hwrs".
+    { iFrame "# %". }
+    wp_apply (wp_Txn__reset with "[$Hwrs $Hptgs]").
+    iIntros "[Hwrs Hptgs]".
+    wp_pures.
+    iApply "HΦ".
+    by iFrame "∗ # %".
+  Qed.
+
+  Theorem wp_Txn__commit_in_abort_future txn tid rds wrs γ τ :
+    is_lnrz_tid γ tid -∗
+    all_prepared γ tid wrs -∗
+    {{{ own_txn_prepared txn tid rds wrs γ τ ∗ own_wabt_tid γ tid }}}
+      Txn__commit #txn
+    {{{ RET #(); False }}}.
+  Proof.
+    iIntros "#Hlnrzed #Hprep" (Φ) "!> [Htxn Hwabt] HΦ".
+    wp_rec.
+
+    (*@ func (txn *Txn) commit() {                                              @*)
+    (*@     trusted_proph.ResolveCommit(txn.proph, txn.ts, txn.wrsp)            @*)
+    (*@                                                                         @*)
+    do 2 iNamed "Htxn". iNamed "Hwrs".
+    do 3 wp_loadField.
+    wp_apply (wp_ResolveCommit with "[$Hwrsp]"); first done.
+    iInv "Hinv" as "> HinvO" "HinvC".
+    iApply ncfupd_mask_intro; first set_solver.
+    iIntros "Hmask".
+    iNamed "HinvO".
+    iDestruct (txnsys_inv_extract_future with "Htxnsys") as (future) "[Hproph Htxnsys]".
+    iFrame "Hproph".
+    iIntros "(%future' & %Hfuture & Hproph)".
+    iMod (txnsys_inv_commit with "Hlnrzed Hprep Htxnsys Hgroups Hrgs Hkeys")
+      as "(Htxnsys & Hgroups & Hrgs & Hkeys & Hcmt)".
+    { by rewrite Hfuture. }
+    (* Obtain contradiction. *)
+    do 2 iNamed "Htxnsys".
+    iDestruct (txn_res_lookup with "Hresm Hcmt") as %Hcmt.
+    iDestruct (wabt_tid_elem_of with "Htidas Hwabt") as %Hwabt.
+    rewrite -Htidas in Hwabt.
+    iDestruct (elem_of_tmodas_partitioned_tids with "Hpart") as %[_ Hnotin].
+    { apply Hwabt. }
+    by specialize (Hnotin _ Hcmt).
+
+    (*@     ts := txn.ts                                                        @*)
+    (*@     wrs := txn.wrs                                                      @*)
+    (*@     for _, gid := range(txn.ptgs) {                                     @*)
+    (*@         gcoord := txn.gcoords[gid]                                      @*)
+    (*@         pwrs := wrs[gid]                                                @*)
+    (*@                                                                         @*)
+    (*@         go func() {                                                     @*)
+    (*@             gcoord.Commit(ts, pwrs)                                     @*)
+    (*@         }()                                                             @*)
+    (*@     }                                                                   @*)
+    (*@                                                                         @*)
+    (*@     txn.reset()                                                         @*)
+    (*@ }                                                                       @*)
+  Qed.
+
+  Theorem wp_Txn__abort txn tid rds wrs γ τ :
+    is_txn_aborted γ tid -∗
+    {{{ own_txn_prepared txn tid rds wrs γ τ ∗ own_wabt_tid γ tid }}}
+      Txn__abort #txn
+    {{{ RET #(); own_txn_uninit txn γ }}}.
+  Proof.
+    iIntros "#Habt" (Φ) "!> [Htxn Hwabt] HΦ".
+    wp_rec.
+
+    (*@ func (txn *Txn) abort() {                                               @*)
+    (*@     trusted_proph.ResolveAbort(txn.proph, txn.ts)                       @*)
+    (*@                                                                         @*)
+    do 2 iNamed "Htxn".
+    do 2 wp_loadField.
+    wp_apply (wp_ResolveAbort); first done.
+    iInv "Hinv" as "> HinvO" "HinvC".
+    iApply ncfupd_mask_intro; first set_solver.
+    iIntros "Hmask".
+    iNamed "HinvO".
+    iDestruct (txnsys_inv_extract_future with "Htxnsys") as (future) "[Hproph Htxnsys]".
+    iFrame "Hproph".
+    iIntros "(%future' & %Hfuture & Hproph)".
+    iMod (txnsys_inv_abort with "Habt Hwabt Htxnsys") as "Htxnsys".
+    { by rewrite Hfuture. }
+    rewrite Hfuture /=.
+    iDestruct (txnsys_inv_merge_future with "Hproph Htxnsys") as "Htxnsys".
+    iMod "Hmask" as "_".
+    iMod ("HinvC" with "[Htxnsys Hkeys Hgroups Hrgs]") as "_"; first by iFrame.
+    iIntros "!> _".
+    wp_pures.
+
+    (*@     ts := txn.ts                                                        @*)
+    (*@     for _, gid := range(txn.ptgs) {                                     @*)
+    (*@                                                                         @*)
+    (*@     txn.reset()                                                         @*)
+    (*@ }                                                                       @*)
+
+
+    (*@     for _, gid := range(txn.ptgs) {                                     @*)
+    (*@         rg := txn.rgs[gid]                                              @*)
+    (*@         rg.Abort(txn.ts)                                                @*)
+    (*@     }                                                                   @*)
+    (*@                                                                         @*)
+    iNamed "Hptgs".
+    do 2 wp_loadField.
+    set P := (λ (_ : u64), own_txn_gcoords txn γ)%I.
+    iDestruct (own_slice_small_acc with "Hptgs") as "[Hptgs HptgsC]".
+    wp_apply (wp_forSlice P with "[] [$Hptgs $Hgcoords]").
+    { (* Loop body. *)
+      clear Φ.
+
+      (*@         gcoord := txn.gcoords[gid]                                      @*)
+      (*@                                                                         @*)
+      iIntros (i gid Φ) "!> (Hgcoords & %Hinbound & %Hgid) HΦ".
+      iNamed "Hgcoords".
+      wp_loadField.
+      assert (Hin : gid ∈ gids_all).
+      { pose proof (subseteq_ptgroups (dom wrs)) as Hdom.
+        apply elem_of_list_lookup_2 in Hgid.
+        clear -Hdom Hgid Hptgs.
+        set_solver.
+      }
+      wp_apply (wp_MapGet with "Hgcoords").
+      iIntros (gcoordP ok) "[%Hgetgcoords Hgcoords]".
+      destruct ok; last first.
+      { apply map_get_false in Hgetgcoords as [Hnone _].
+        by rewrite -not_elem_of_dom Hdomgcoords in Hnone.
+      }
+      apply map_get_true in Hgetgcoords.
+      (*@         go func() {                                                     @*)
+      (*@             gcoord.Abort(ts)                                            @*)
+      (*@         }()                                                             @*)
+      (*@     }                                                                   @*)
+      (*@                                                                         @*)
+      wp_pures.
+      iDestruct (big_sepM_lookup with "Hgcoordsabs") as "Hgcoordabs"; first apply Hgetgcoords.
+      wp_apply wp_fork.
+      { wp_apply (wp_GroupCoordinator__Abort with "[] Hgcoordabs").
+        { rewrite Htsword. by iFrame "Habt". }
+        done.
+      }
+      iApply "HΦ".
+      iFrame "∗ # %".
+    }
+    iIntros "[Hgcoods Hptgs]". subst P. simpl.
+    iDestruct ("HptgsC" with "Hptgs") as "Hptgs".
+    iAssert (own_txn_ptgs txn ptgs)%I with "[$HptgsS $Hptgs]" as "Hptgs"; first done.
+
+    (*@     txn.reset()                                                         @*)
+    (*@ }                                                                       @*)
+    wp_apply (wp_Txn__reset with "[$Hwrs $Hptgs]").
+    iIntros "[Hwrs Hptgs]".
+    wp_pures.
+    iApply "HΦ".
+    by iFrame "∗ # %".
+  Qed.
+
+  Theorem wp_Txn__abort_in_commit_future txn tid rds wrsphys wrsproph γ τ :
+    is_txn_aborted γ tid -∗
+    {{{ own_txn_prepared txn tid rds wrsphys γ τ ∗ own_cmt_tmod γ tid wrsproph }}}
+      Txn__abort #txn
+    {{{ RET #(); False }}}.
+  Proof.
+    iIntros "#Habt" (Φ) "!> [Htxn Htidc] HΦ".
+    wp_rec.
+
+    (*@ func (txn *Txn) abort() {                                               @*)
+    (*@     trusted_proph.ResolveAbort(txn.proph, txn.ts)                       @*)
+    (*@                                                                         @*)
+    do 2 iNamed "Htxn".
+    do 2 wp_loadField.
+    wp_apply (wp_ResolveAbort); first done.
+    iInv "Hinv" as "> HinvO" "HinvC".
+    iApply ncfupd_mask_intro; first set_solver.
+    iIntros "Hmask".
+    iNamed "HinvO". do 2 iNamed "Htxnsys".
+    iFrame "Hproph".
+    iIntros "(%future' & %Hfuture & Hproph)".
+    (* Prove [tid] must not have committed. *)
+    iDestruct (txn_res_lookup with "Hresm Habt") as %Habt.
+    iDestruct (cmt_tmod_lookup with "Htidcs Htidc") as %Htidc.
+    specialize (Htidcs _ _ Htidc). simpl in Htidcs.
+    destruct Htidcs as [Hwc | Hcmt]; last first.
+    { by rewrite Hcmt in Habt. }
+    specialize (Hcf _ _ Hwc). simpl in Hcf.
+    destruct Hcf as (lp & ls & Hfc & _).
+    assert (Hhead : head_abort future tid).
+    { by rewrite Hfuture. }
+    destruct (first_commit_head_abort _ _ _ _ _ Hfc Hhead) as [].
+
+    (*@     ts := txn.ts                                                        @*)
+    (*@     for _, gid := range(txn.ptgs) {                                     @*)
+    (*@         gcoord := txn.gcoords[gid]                                      @*)
+    (*@                                                                         @*)
+    (*@         go func() {                                                     @*)
+    (*@             gcoord.Abort(ts)                                            @*)
+    (*@         }()                                                             @*)
+    (*@     }                                                                   @*)
+    (*@                                                                         @*)
+    (*@     txn.reset()                                                         @*)
+    (*@ }                                                                       @*)
+  Qed.
+
+  Theorem wp_Txn__cancel txn tid rds γ τ :
+    {{{ own_txn txn tid rds γ τ ∗ own_wabt_tid γ tid ∗ own_txn_reserved_wrs γ tid }}}
+      Txn__cancel #txn
+    {{{ RET #(); own_txn_uninit txn γ }}}.
+  Proof.
+    iIntros (Φ) "(Htxn & Habt & Hwrsexcl) HΦ".
+    wp_rec.
+
+    (*@ func (txn *Txn) cancel() {                                              @*)
+    (*@     trusted_proph.ResolveAbort(txn.proph, txn.ts)                       @*)
+    (*@                                                                         @*)
+    do 2 iNamed "Htxn".
+    do 2 wp_loadField.
+    wp_apply (wp_ResolveAbort); first done.
+    iInv "Hinv" as "> HinvO" "HinvC".
+    iApply ncfupd_mask_intro; first set_solver.
+    iIntros "Hmask".
+    iNamed "HinvO".
+    iDestruct (txnsys_inv_extract_future with "Htxnsys") as (future) "[Hproph Htxnsys]".
+    iFrame "Hproph".
+    iIntros "(%future' & %Hfuture & Hproph)".
+    iMod (txnsys_inv_cancel with "Habt Hwrsexcl Htxnsys") as "Htxnsys".
+    { by rewrite Hfuture. }
+    rewrite Hfuture /=.
+    iDestruct (txnsys_inv_merge_future with "Hproph Htxnsys") as "Htxnsys".
+    iMod "Hmask" as "_".
+    iMod ("HinvC" with "[Htxnsys Hkeys Hgroups Hrgs]") as "_"; first by iFrame.
+    iIntros "!> _".
+
+    (*@     txn.reset()                                                         @*)
+    (*@ }                                                                       @*)
+    wp_apply (wp_Txn__reset with "[$Hwrs $Hptgs]").
+    iIntros "[Hwrs Hptgs]".
+    wp_pures.
+    iApply "HΦ".
+    by iFrame "∗ # %".
+  Qed.
+
+  Theorem wp_Txn__cancel_in_commit_future txn tid rds γ τ :
+    {{{ own_txn txn tid rds γ τ ∗ (∃ m, own_cmt_tmod γ tid m) ∗ own_txn_reserved_wrs γ tid }}}
+      Txn__cancel #txn
+    {{{ RET #(); False }}}.
+  Proof.
+    iIntros (Φ) "(Htxn & [%m Htidc] & Hwrsexcl) HΦ".
+    wp_rec.
+
+    (*@ func (txn *Txn) cancel() {                                              @*)
+    (*@     trusted_proph.ResolveAbort(txn.proph, txn.ts)                       @*)
+    (*@                                                                         @*)
+    do 2 iNamed "Htxn".
+    do 2 wp_loadField.
+    wp_apply (wp_ResolveAbort); first done.
+    iInv "Hinv" as "> HinvO" "HinvC".
+    iApply ncfupd_mask_intro; first set_solver.
+    iIntros "Hmask".
+    iNamed "HinvO". do 2 iNamed "Htxnsys".
+    iFrame "Hproph".
+    iIntros "(%future' & %Hfuture & Hproph)".
+    (* Obtain [tmods !! tid = Some m]. *)
+    iDestruct (cmt_tmod_lookup with "Htidcs Htidc") as %Htidc.
+    specialize (Htidcs _ _ Htidc). simpl in Htidcs.
+    (* Prove [resm !! tid = Some (ResCommitted m)] impossible, i.e., [tid] not committed yet. *)
+    destruct Htidcs as [Htmodcs | Hcmt]; last first.
+    { iDestruct (big_sepM_lookup with "Hvr") as "Hvc"; first apply Hcmt.
+      iDestruct "Hvc" as "[Hwrsrcpt _]".
+      (* Contradicting facts:
+       * 1. Txn still owns exclusively the write-set (which is true before prepare).
+       * Represented as [Hwrsexcl] from the precondition.
+       * 2. Txn has set the write-set and given up the ability to change
+       * (which is true after prepare). Represented as [Hwrsrcpt].
+       *)
+      by iDestruct (txn_oneshot_wrs_agree with "Hwrsexcl Hwrsrcpt") as %Hcontra.
+    }
+    (* Obtain [first_commit]. *)
+    specialize (Hcf _ _ Htmodcs). simpl in Hcf.
+    destruct Hcf as (lp & ls & Hfc & _).
+    (* Obtain contradiction from [first_commit] and [head_abort]. *)
+    assert (Hha : head_abort future tid).
+    { by rewrite Hfuture /head_abort /=. }
+    destruct (first_commit_head_abort _ _ _ _ _ Hfc Hha).
+
+    (*@     txn.reset()                                                         @*)
+    (*@ }                                                                       @*)
+  Qed.
+
+  Theorem wp_Txn__begin (txn : loc) γ :
+    ⊢ {{{ own_txn_uninit txn γ }}}
+      <<< ∀∀ (ts : nat), own_largest_ts γ ts >>>
+        Txn__begin #txn @ ↑tsNS
+      <<< ∃∃ (ts' : nat), own_largest_ts γ ts' ∗ ⌜(ts < ts')%nat⌝ >>>
+      {{{ RET #(); own_txn_init txn ts' γ }}}.
+  Proof.
+    (*@ func (txn *Txn) begin() {                                               @*)
+    (*@     // TODO                                                             @*)
+    (*@     // Ghost action: Linearize.                                         @*)
+    (*@     txn.ts = GetTS()                                                    @*)
+    (*@ }                                                                       @*)
+  Admitted.
+
+  Theorem wp_Txn__prepare txn tid rds wrs γ τ :
+    {{{ own_txn_stable txn tid rds wrs γ τ }}}
+      Txn__prepare #txn
+    {{{ (status : txnphase), RET #(txnphase_to_u64 status); 
+        own_txn_prepared txn tid rds wrs γ τ ∗ safe_txnphase γ tid status
+    }}}.
+  Proof.
+    iIntros (Φ) "Htxn HΦ".
+    wp_rec.
+
+    (*@ func (txn *Txn) prepare() uint64 {                                      @*)
+    (*@     // Compute the participant groups.                                  @*)
+    (*@     txn.setptgs()                                                       @*)
+    (*@                                                                         @*)
+    iNamed "Htxn".
+    wp_apply (wp_Txn__setptgs with "[$Hwrs $Hptgs]").
+    iIntros "Hptgs".
+    iDestruct "Hptgs" as (ptgs) "(Hwrs & Hptgs & %Hptgs)".
+
+    (*@     // TODO: init the group coordinator                                 @*)
+    (*@                                                                         @*)
+    (*@     ts := txn.ts                                                        @*)
+    (*@     ptgs := txn.ptgs                                                    @*)
+    (*@                                                                         @*)
+    iNamed "Htxn". iNamed "Hptgs".
+    do 2 wp_loadField.
+
+    (*@     // An alternative (and more elegant) design would be using a wait-groups, but @*)
+    (*@     // the CV approach has the advantage of early abort: If the transaction @*)
+    (*@     // fails to prepare on one of the participant groups (e.g., due to conflict @*)
+    (*@     // with another transaction), then the CV approach can "short-circuiting" to @*)
+    (*@     // aborting the entire transaction, whereas the WaitGroup approach would @*)
+    (*@     // have to wait until all groups reach their own prepare decisions. @*)
+    (*@     mu := new(sync.Mutex)                                               @*)
+    (*@     cv := sync.NewCond(mu)                                              @*)
+    (*@     var np uint64 = 0                                                   @*)
+    (*@     var st uint64 = tulip.TXN_PREPARED                                  @*)
+    (*@                                                                         @*)
+    wp_apply wp_new_free_lock.
+    iIntros (muP) "Hfree".
+    wp_apply (wp_newCond' with "Hfree").
+    iIntros (cvP) "[Hfree #Hcv]".
+    wp_apply wp_ref_to; first by auto.
+    iIntros (npP) "HnpP".
+    wp_apply wp_ref_to; first by auto.
+    iIntros (stP) "HstP".
+    wp_pures.
+    (* Allocate exclusive tokens to prove freshness of response. *)
+    iApply fupd_wp.
+    iMod (local_gid_tokens_alloc (ptgroups (dom wrs))) as (α) "Htks".
+    iModIntro.
+    (* Establish the lock invariant. *)
+    set I := (∃ (np : u64) (st : txnphase) (gids : gset u64),
+                 "HnpP" ∷ npP ↦[uint64T] #np ∗
+                 "HstP" ∷ stP ↦[uint64T] #(txnphase_to_u64 st) ∗
+                 "Htks" ∷ ([∗ set] gid ∈ gids, local_gid_token α gid) ∗
+                 "#Hst" ∷ (match st with
+                           | TxnPrepared => [∗ set] gid ∈ gids, is_group_prepared γ gid tid
+                           | TxnCommitted => (∃ wrs, is_txn_committed γ tid wrs)
+                           | TxnAborted => is_txn_aborted γ tid
+                           end) ∗
+                 "%Hgidsincl" ∷ ⌜gids ⊆ ptgroups (dom wrs)⌝ ∗
+                 "%Hsizegids" ∷ ⌜size gids = uint.nat np⌝)%I.
+    iApply fupd_wp.
+    iMod (alloc_lock tulipNS _ _ I with "Hfree [HnpP HstP]") as "#Hmu".
+    { iModIntro.
+      iExists (W64 0), TxnPrepared, ∅.
+      iFrame.
+      iSplit; first by iApply big_sepS_empty.
+      iSplit; first by iApply big_sepS_empty.
+      done.
+    }
+    iModIntro.
+
+    (*@     // Some notes about the concurrency reasoning here:                 @*)
+    (*@     //                                                                  @*)
+    (*@     // 1. Even though at any point the group coordinators are assigned  @*)
+    (*@     // exclusively to @txn.ts, the fact that it is reused (for performance @*)
+    (*@     // reason: connection can be established only once for each @Txn object) @*)
+    (*@     // means that the associated timestamp is not exposed in the representation @*)
+    (*@     // predicate. Hence, we'll need a fractional RA to remember that the group @*)
+    (*@     // coordinators are assigned to @txn.ts during the course of @txn.prepare. @*)
+    (*@     //                                                                  @*)
+    (*@     // 2. To establish sufficient proof that @txn.ts can finalize, we need to @*)
+    (*@     // maintain the following the lock invariant:                       @*)
+    (*@     // There exists a set G of group IDs:                               @*)
+    (*@     // (a) @st associated with the right txn tokens; for @st = TXN_PREPARED, in @*)
+    (*@     // particular, all groups in G must have prepared;                  @*)
+    (*@     // (b) size(G) = @np;                                               @*)
+    (*@     // (c) exclusive tokens over G, allowing a coordinator to prove uniqueness @*)
+    (*@     // when adding its result, and thereby re-esbalish property (b).    @*)
+    (*@                                                                         @*)
+    (*@     // Try to prepare transaction @tcoord.ts on each group.             @*)
+    (*@     for _, gid := range(ptgs) {                                         @*)
+    (*@                                                                         @*)
+    do 2 iNamed "Hwrs".
+    iDestruct "Hpwrsm" as "#Hpwrsm".
+    wp_loadField.
+    set P := (λ (i : u64),
+                "HpwrsmP" ∷ own_map wrsP (DfracOwn 1) pwrsmP ∗
+                "Hgcoords" ∷ own_txn_gcoords txn γ ∗
+                "Htks" ∷ [∗ set] gid ∈ list_to_set (drop (uint.nat i) ptgs), local_gid_token α gid)%I.
+    iDestruct (own_slice_small_acc with "Hptgs") as "[Hptgs HptgsC]".
+    iDestruct (own_slice_small_sz with "Hptgs") as %Hlenptgs.
+    wp_apply (wp_forSlice P with "[] [$Hptgs $HpwrsmP $Hgcoords Htks]"); last first; first 1 last.
+    { by rewrite uint_nat_W64_0 drop_0 Hptgs. }
+    { clear Φ.
+
+      (*@         gcoord := txn.gcoords[gid]                                      @*)
+      (*@         pwrs := txn.wrs[gid]                                            @*)
+      (*@                                                                         @*)
+      iIntros (i gid Φ) "!> (HP & %Hinbound & %Hgid) HΦ".
+      iNamed "HP". iNamed "Hgcoords".
+      wp_loadField.
+      assert (Hin : gid ∈ gids_all).
+      { pose proof (subseteq_ptgroups (dom wrs)) as Hdom.
+        apply elem_of_list_lookup_2 in Hgid.
+        clear -Hdom Hgid Hptgs.
+        set_solver.
+      }
+      wp_apply (wp_MapGet with "Hgcoords").
+      iIntros (gcoordP ok) "[%Hgetgcoords Hgcoords]".
+      destruct ok; last first.
+      { apply map_get_false in Hgetgcoords as [Hnone _].
+        by rewrite -not_elem_of_dom Hdomgcoords in Hnone.
+      }
+      apply map_get_true in Hgetgcoords.
+      wp_apply (wp_MapGet with "HpwrsmP").
+      iIntros (pwrsP ok) "[%Hgetwrs HpwrsmP]".
+      destruct ok; last first.
+      { apply map_get_false in Hgetwrs as [Hnotin _].
+        by rewrite -not_elem_of_dom Hdomwrs in Hnotin.
+      }
+      apply map_get_true in Hgetwrs.
+      iAssert (⌜is_Some (pwrsm !! gid)⌝)%I as %[pwrs Hpwrs].
+      { iDestruct (big_sepM2_dom with "Hpwrsm") as %Hdom.
+        iPureIntro.
+        by rewrite -elem_of_dom -Hdom elem_of_dom.
+      }
+      iDestruct (big_sepM2_lookup_acc with "Hpwrsm") as "[Hpwrs HpwrsmC]"; [done | done |].
+      wp_pures.
+      assert (Hvg : gid ∈ ptgroups (dom wrs)).
+      { rewrite -Hptgs elem_of_list_to_set. by apply elem_of_list_lookup_2 in Hgid. }
+
+      (*@         go func() {                                                     @*)
+      (*@                                                                         @*)
+      iDestruct (big_sepM_lookup with "Hgcoordsabs") as "Hgcoordabs"; first apply Hgetgcoords.
+      rewrite (drop_S _ _ _ Hgid) list_to_set_cons big_sepS_insert; last first.
+      { rewrite not_elem_of_list_to_set. intros Hgidin.
+        clear -Hgid Hgidin Hnd.
+        rewrite -(take_drop_middle _ _ _ Hgid) in Hnd.
+        apply NoDup_app in Hnd as (_ & _ & Hnd).
+        by apply NoDup_cons in Hnd as [? _].
+      }
+      iDestruct "Htks" as "[Htk Htks]".
+      wp_apply (wp_fork with "[Htk]").
+      { (* Forked thread. *)
+
+        (*@             stg, ok := gcoord.Prepare(ts, ptgs, pwrs)                   @*)
+        (*@                                                                         @*)
+        iModIntro.
+        wp_apply (wp_GroupCoordinator__Prepare with "Hgcoordabs").
+        iIntros (stg ok) "#Hsafe".
+        wp_pures.
+
+        (*@             if ok {                                                     @*)
+        (*@                 mu.Lock()                                               @*)
+        (*@                 if stg == tulip.TXN_PREPARED {                          @*)
+        (*@                     np += 1                                             @*)
+        (*@                 } else {                                                @*)
+        (*@                     st = stg                                            @*)
+        (*@                 }                                                       @*)
+        (*@                 mu.Unlock()                                             @*)
+        (*@                 cv.Signal()                                             @*)
+        (*@             }                                                           @*)
+        (*@                                                                         @*)
+        destruct ok; wp_pures.
+        { wp_apply (wp_Mutex__Lock with "Hmu").
+          iIntros "[Hlocked HI]".
+          iNamed "HI".
+          assert (Hszgids : (size gids ≤ size gids_all)%nat).
+          { apply subseteq_size. etrans; [apply Hgidsincl | apply subseteq_ptgroups]. }
+          pose proof size_gids_all as Hszgidsall.
+          wp_pures.
+          (* Prove [safe_txn_pwrs] used in invariance of PREPARE and UNPREPARE. *)
+          iAssert (safe_txn_pwrs γ gid tid pwrs)%I as "#Hsafepwrs".
+          { iFrame "Htxnwrs".
+            iPureIntro.
+            specialize (Hwrsg _ _ Hpwrs). simpl in Hwrsg.
+            pose proof (elem_of_ptgroups_non_empty _ _ Hvg) as Hne.
+            rewrite -Hwrsg in Hne.
+            done.
+          }
+          case_bool_decide as Hstg; wp_pures.
+          { (* Case [TxnPrepared]. *)
+            wp_load. wp_store.
+            destruct stg; [| done | done].
+            rewrite Htsword /=.
+            iAssert (|={⊤}=> is_group_prepared γ gid tid)%I as "Hprepared".
+            { iInv "Hinv" as "> HinvO" "HinvC".
+              iNamed "HinvO".
+              iDestruct (big_sepS_elem_of_acc with "Hgroups") as "[Hgroup HgroupsC]".
+              { apply Hin. }
+              iDestruct (big_sepS_elem_of_acc with "Hrgs") as "[Hrg HrgsC]".
+              { apply Hin. }
+              iDestruct "Hsafe" as "[Hqp Hqv]".
+              iMod (group_inv_prepare with "Hqv Hqp Hsafepwrs Htxnsys Hkeys Hrg Hgroup")
+                as "(Htxnsys & Hkeys & Hrg & Hgroup & #Hprepared)".
+              iDestruct ("HrgsC" with "Hrg") as "Hrgs".
+              iDestruct ("HgroupsC" with "Hgroup") as "Hgroups".
+              iMod ("HinvC" with "[$Htxnsys $Hkeys $Hgroups $Hrgs]") as "_".
+              done.
+            }
+            iMod "Hprepared" as "#Hprepared".
+            wp_apply (wp_Mutex__Unlock with "[-]").
+            { iFrame "Hmu Hlocked HnpP HstP".
+              iModIntro.
+              iExists ({[gid]} ∪ gids).
+              iAssert (⌜gid ∉ gids⌝)%I as %Hnotin.
+              { iIntros (Hgidin).
+                iDestruct (big_sepS_elem_of with "Htks") as "Htk'"; first apply Hgidin.
+                by iDestruct (local_gid_token_ne with "Htk Htk'") as %?.
+              }
+              iSplitL "Htk Htks".
+              { iApply (big_sepS_insert_2 with "Htk Htks"). }
+              iSplit.
+              { destruct st; [| done | done].
+                by iApply big_sepS_insert_2.
+              }
+              iPureIntro.
+              { split.
+                { clear -Hgidsincl Hvg. set_solver. }
+                { rewrite size_union; last set_solver.
+                  rewrite size_singleton Hsizegids.
+                  clear -Hszgids Hszgidsall Hsizegids. word.
+                }
+              }
+            }
+            by wp_apply (wp_Cond__Signal with "Hcv").
+          }
+          { wp_store.
+            destruct stg eqn:Hstgeq; first done.
+            { (* Case [TxnCommitted]. *)
+              wp_apply (wp_Mutex__Unlock with "[-]").
+              { iFrame "Hmu Hlocked ∗ # %". by rewrite Htsword. }
+              by wp_apply (wp_Cond__Signal with "Hcv").
+            }
+            { (* Case [TxnAborted]. *)
+              rewrite Htsword.
+              iAssert (|={⊤}=> is_txn_aborted γ tid)%I as "Habted".
+              { iDestruct "Hsafe" as "[? | Hsafe]"; first done.
+                iInv "Hinv" as "> HinvO" "HinvC".
+                iNamed "HinvO".
+                iDestruct (big_sepS_elem_of_acc with "Hgroups") as "[Hgroup HgroupsC]".
+                { apply Hin. }
+                iDestruct (big_sepS_elem_of_acc with "Hrgs") as "[Hrg HrgsC]".
+                { apply Hin. }
+                iMod (txnsys_group_inv_unprepare with "Hsafe Hsafepwrs Hrg Hgroup Htxnsys")
+                  as "(Hrg & Hgroup & Htxnsys & #Habted)".
+                iDestruct ("HrgsC" with "Hrg") as "Hrgs".
+                iDestruct ("HgroupsC" with "Hgroup") as "Hgroups".
+                iMod ("HinvC" with "[$Htxnsys $Hkeys $Hgroups $Hrgs]") as "_".
+                done.
+              }
+              iMod "Habted" as "#Habted".
+              wp_apply (wp_Mutex__Unlock with "[-]").
+              { iFrame "Hmu Hlocked ∗ # %". }
+              by wp_apply (wp_Cond__Signal with "Hcv").
+            }
+          }
+        }
+
+        (*@             // @ok = false means that the group coordinator has already been @*)
+        (*@             // assigned to a different transaction, implying nothing is waiting @*)
+        (*@             // on the CV.                                               @*)
+        (*@         }()                                                             @*)
+        (*@     }                                                                   @*)
+        (*@                                                                         @*)
+        done.
+      }
+
+      iApply "HΦ".
+      iFrame "∗ # %".
+      rewrite uint_nat_word_add_S; last first.
+      { clear -Hinbound. word. }
+      done.
+    }
+
+    (*@     mu.Lock()                                                           @*)
+    (*@     // Wait until either status is no longer TXN_PREPARED or all participant @*)
+    (*@     // groups have responded.                                           @*)
+    (*@     for st == tulip.TXN_PREPARED && np != uint64(len(ptgs)) {           @*)
+    (*@         cv.Wait()                                                       @*)
+    (*@     }                                                                   @*)
+    (*@                                                                         @*)
+    iIntros "[HP Hptgs]".
+    subst P. iNamed "HP".
+    wp_apply (wp_Mutex__Lock with "Hmu").
+    iIntros "[Hlocked HI]".
+    wp_pures.
+    set P := (λ cont : bool,
+                ∃ (np : u64) (st : txnphase) (gids : gset u64),
+                  "HnpP" ∷ npP ↦[uint64T] #np ∗
+                  "HstP" ∷ stP ↦[uint64T] #(txnphase_to_u64 st) ∗
+                  "Htks" ∷ ([∗ set] gid ∈ gids, local_gid_token α gid) ∗
+                  "Hlocked" ∷ locked #muP ∗
+                  "#Hst" ∷ (match st with
+                            | TxnPrepared => [∗ set] gid ∈ gids, is_group_prepared γ gid tid
+                            | TxnCommitted => (∃ wrs, is_txn_committed γ tid wrs)
+                            | TxnAborted => is_txn_aborted γ tid
+                            end) ∗
+                  "%Hgidsincl" ∷ ⌜gids ⊆ ptgroups (dom wrs)⌝ ∗
+                  "%Hsizegids" ∷ ⌜size gids = uint.nat np⌝ ∗
+                  "%Hcond"     ∷ ⌜(if cont
+                                   then True
+                                   else match st with
+                                        | TxnPrepared => uint.nat np = length ptgs
+                                        | _ => True
+                                        end)⌝)%I.
+    wp_apply (wp_forBreak_cond P with "[] [Hlocked HI]"); last first; first 1 last.
+    { iNamed "HI". iFrame "∗ # %". }
+    { clear Φ.
+      iIntros (Φ) "!> HP HΦ".
+      iNamed "HP".
+      wp_load.
+      wp_pures.
+      case_bool_decide as Hprepared; wp_pures.
+      { wp_load.
+        wp_apply wp_slice_len.
+        wp_pures.
+        case_bool_decide as Hsize; wp_pures.
+        { iApply "HΦ".
+          iFrame "∗ # %".
+          iPureIntro.
+          destruct st; try done.
+          inv Hsize.
+          clear -Hlenptgs. done.
+        }
+        wp_apply (wp_Cond__Wait with "[-HΦ]").
+        { by iFrame "Hcv Hmu Hlocked ∗ # %". }
+        iIntros "[Hlocked HI]".
+        wp_pures.
+        iApply "HΦ".
+        iClear "Hst".
+        iNamed "HI".
+        by iFrame "∗ # %".
+      }
+      iApply "HΦ".
+      iFrame "∗ # %".
+      iPureIntro.
+      by destruct st.
+    }
+    iClear "Htks".
+    iNamed 1.
+        
+    (*@     status := st                                                        @*)
+    (*@     mu.Unlock()                                                         @*)
+    (*@                                                                         @*)
+    wp_load. wp_pures.
+    wp_apply (wp_Mutex__Unlock with "[Hlocked HnpP HstP Htks]").
+    { by iFrame "Hmu Hlocked ∗ # %". }
+
+    (*@     return status                                                       @*)
+    (*@ }                                                                       @*)
+    wp_pures.
+    iApply "HΦ".
+    iAssert (safe_txnphase γ tid st)%I as "#Hsafe".
+    { destruct st; [| done | done].
+      simpl.
+      iFrame "Htxnwrs".
+      assert (gids = ptgroups (dom wrs)) as ->; last done.
+      apply set_subseteq_size_eq; first apply Hgidsincl.
+      rewrite -Hptgs size_list_to_set; last apply Hnd.
+      clear -Hsizegids Hcond. lia.
+    }
+    iDestruct ("HptgsC" with "Hptgs") as "Hptgs".
+    by iFrame "Hsafe ∗ # %".
+  Qed.
+
+  Definition body_spec
+    (body : val) (txn : loc) tid r
+    (P : dbmap -> Prop) (Q : dbmap -> dbmap -> Prop)
+    (Rc : dbmap -> dbmap -> iProp Σ) (Ra : dbmap -> iProp Σ)
+    γ τ : iProp Σ :=
+    ∀ Φ,
+    own_txn txn tid r γ τ ∗ ⌜P r⌝ ∗ txnmap_ptstos τ r -∗
+    (∀ ok : bool,
+       (own_txn txn tid r γ τ ∗
+        if ok
+        then ∃ w, ⌜Q r w ∧ dom r = dom w⌝ ∗ (Rc r w ∧ Ra r) ∗ txnmap_ptstos τ w
+        else Ra r) -∗ Φ #ok) -∗
+    WP body #txn {{ v, Φ v }}.
+
+  Theorem wp_Txn__Run
+    txn (body : val)
+    (P : dbmap -> Prop) (Q : dbmap -> dbmap -> Prop)
+    (Rc : dbmap -> dbmap -> iProp Σ) (Ra : dbmap -> iProp Σ) γ :
+    (∀ r w, (Decision (Q r w))) ->
+    ⊢ {{{ own_txn_uninit txn γ ∗ (∀ tid r τ, body_spec body txn tid r P Q Rc Ra γ τ) }}}
+      <<< ∀∀ (r : dbmap), ⌜P r ∧ dom r ⊆ keys_all⌝ ∗ own_db_ptstos γ r >>>
+        Txn__Run #txn body @ ↑sysNS
+      <<< ∃∃ (ok : bool) (w : dbmap), if ok then ⌜Q r w⌝ ∗ own_db_ptstos γ w else own_db_ptstos γ r >>>
+      {{{ RET #ok; own_txn_uninit txn γ ∗ if ok then Rc r w else Ra r }}}.
+  Proof.
+    iIntros (Hdec) "!>".
+    iIntros (Φ) "[Htxn Hbody] HAU".
+    wp_rec. wp_pures.
+
+    (*@ func (txn *Txn) Run(body func(txn *Txn) bool) bool {                    @*)
+    (*@     txn.begin()                                                         @*)
+    (*@                                                                         @*)
+    iAssert (∃ p, know_tulip_inv_with_proph γ p)%I as (p) "#Hinv".
+    { do 2 iNamed "Htxn". iFrame "Hinv". }
+    wp_apply (wp_Txn__begin with "[-Hbody HAU]").
+    { iFrame "∗ # %". }
+    iInv "Hinv" as "> HinvO" "HinvC".
+    iMod (ncfupd_mask_subseteq (⊤ ∖ ↑sysNS)) as "Hclose"; first solve_ndisj.
+    iMod "HAU" as (rds) "[[[%HP %Hdomr] Hdbpts] HAUC]".
+    iModIntro.
+    iNamed "HinvO".
+    iDestruct (txnsys_inv_expose_future_extract_ts with "Htxnsys")
+      as (future ts) "[Htxnsys Hts]".
+    (* Prove [key_inv] are linearizable after [ts]. *)
+    iDestruct (keys_inv_before_linearize with "Hkeys Hts") as "[Hkeys Hts]".
+    iExists ts.
+    (* Pass [ts_auth γ ts] to the underlying layer. *)
+    iFrame "Hts".
+    iIntros (tid) "[Hts %Htidgt]".
+    iDestruct (largest_ts_witness with "Hts") as "#Htidlb".
+
+    pose proof (peek_spec future tid) as Hpeek.
+    set form := peek _ _ in Hpeek.
+    set Qr := λ m, Q rds (m ∪ rds) ∧ dom m ⊆ dom rds.
+    destruct (decide (incorrect_fcc Qr form)) as [Hifcc | HQ].
+    { (* Case: Abort branch. *)
+      iMod (txnsys_inv_linearize_abort form Q with "Htidlb Hdbpts Htxnsys Hkeys")
+        as "(Hdbpts & Htxnsys & Hkeys & Htida & Hwrsexcl & Hclients & #HQ & #Hlnrzs & #Hlnrzed)".
+      { apply Hdomr. }
+      { apply Htidgt. }
+      { apply Hpeek. }
+      { done. }
+      (* Choose the will-abort branch. Use [∅] as placeholder. *)
+      iMod ("HAUC" $! false ∅ with "Hdbpts") as "HΦ".
+      iMod "Hclose" as "_".
+      iMod ("HinvC" with "[Hts Htxnsys Hkeys Hgroups Hrgs]") as "_".
+      { iNamed "Htxnsys". iFrame "∗ # %". }
+      (* Allocate transaction local view [txnmap_ptstos τ r]. *)
+      iMod (txnmap_alloc rds) as (τ) "[Htxnmap Htxnpts]".
+      iIntros "!> Htxn".
+      iAssert (own_txn txn tid rds γ τ)%I with "[Htxn Htxnmap]" as "Htxn".
+      { iClear "Hinv". do 2 iNamed "Htxn".
+        iExists _, ∅.
+        rewrite map_empty_union.
+        by iFrame "∗ # %".
+      }
+
+      (*@     cmt := body(txn)                                                    @*)
+      (*@                                                                         @*)
+      wp_apply ("Hbody" with "[$Htxn $Htxnpts]"); first done.
+      iIntros (cmt) "[Htxn Hpts]".
+
+      (*@     if !cmt {                                                           @*)
+      (*@         // This transaction has not really requested to prepare yet, so no @*)
+      (*@         // cleanup tasks are required.                                  @*)
+      (*@         txn.cancel()                                                    @*)
+      (*@         return false                                                    @*)
+      (*@     }                                                                   @*)
+      (*@                                                                         @*)
+      wp_if_destruct.
+      { wp_apply (wp_Txn__cancel with "[$Htxn $Htida $Hwrsexcl]").
+        iIntros "Htxn".
+        wp_pures.
+        iApply "HΦ".
+        by iFrame.
+      }
+
+      (*@     status := txn.prepare()                                             @*)
+      (*@                                                                         @*)
+      iDestruct "Hpts" as (w) "([%HQ %Hdomw] & [_ HRa] & Hpts)".
+      iAssert (|={⊤}=> ∃ wrst, own_txn_stable txn tid rds wrst γ τ)%I
+        with "[Htxn Hwrsexcl Hpts]" as "Htxn".
+      { iClear "Hinv". iNamed "Htxn".
+        iDestruct (txnmap_subseteq with "Htxnmap Hpts") as %Hsubseteq.
+        unshelve epose proof (subseteq_dom_eq _ _ Hsubseteq _) as Heq.
+        { clear -Hincl Hdomw. set_solver. }
+        subst w.
+        iInv "Hinv" as "> HinvO" "HinvC".
+        iNamed "HinvO".
+        iMod (txnsys_inv_preprepare with "HQ Hwrsexcl Htxnsys") as "[Htxnsys Hwrsrcpt]".
+        { apply Hvts. }
+        { apply Hvwrs. }
+        { done. }
+        iMod ("HinvC" with "[$Htxnsys $Hkeys $Hgroups $Hrgs]") as "_".
+        iFrame "∗ # %".
+        do 2 iNamed "Hwrs".
+        iFrame "∗ %".
+        rewrite -big_sepM2_fupd.
+        iApply (big_sepM2_mono with "Hpwrsm").
+        iIntros (g r m Hr Hm) "Hm".
+        by iMod (own_map_persist with "Hm") as "Hm".
+      }
+      iMod "Htxn" as (wrst) "Htxn".
+      wp_apply (wp_Txn__prepare with "Htxn").
+      iIntros (status) "[Htxn Hstatus]".
+
+      (*@     if status == TXN_COMMITTED {                                        @*)
+      (*@         // A backup coordinator must have committed this transaction, so simply @*)
+      (*@         // reset the write-set here.                                    @*)
+      (*@         txn.reset()                                                     @*)
+      (*@         return true                                                     @*)
+      (*@     }                                                                   @*)
+      (*@                                                                         @*)
+      wp_if_destruct.
+      { destruct status eqn:Hstatus; [done | | done]. clear Heqb.
+        subst status.
+        iDestruct "Hstatus" as (wrs) "Hcmt".
+        (* Obtain a contradiction from [Hcmt] and [Htida]. *)
+        iApply fupd_wp.
+        iInv "Hinv" as "> HinvO" "HinvC".
+        iNamed "HinvO". do 2 iNamed "Htxnsys".
+        iDestruct (txn_res_lookup with "Hresm Hcmt") as %Hcmt.
+        iDestruct (wabt_tid_elem_of with "Htidas Htida") as %Hwabt.
+        rewrite -Htidas in Hwabt.
+        iDestruct (elem_of_tmodas_partitioned_tids with "Hpart") as %[_ Hnotin].
+        { apply Hwabt. }
+        by specialize (Hnotin _ Hcmt).
+      }
+      rename Heqb into Hstatusnc.
+
+      (*@     if status == TXN_ABORTED {                                          @*)
+      (*@         // Ghost action: Abort this transaction.                        @*)
+      (*@         txn.abort()                                                     @*)
+      (*@         return false                                                    @*)
+      (*@     }                                                                   @*)
+      (*@                                                                         @*)
+      wp_if_destruct.
+      { destruct status eqn:Hstatus; [done | done |]. clear Heqb.
+        subst status.
+        wp_apply (wp_Txn__abort with "Hstatus [$Htxn $Htida]").
+        iIntros "Htxn".
+        wp_pures.
+        iApply "HΦ".
+        by iFrame.
+      }
+      rename Heqb into Hstatusna.
+
+      (*@     // Ghost action: Commit this transaction.                           @*)
+      (*@     txn.commit()                                                        @*)
+      (*@     return true                                                         @*)
+      (*@ }                                                                       @*)
+      destruct status; [| done | done]. simpl. clear Hstatusnc Hstatusna.
+      iDestruct "Hstatus" as (wrs) "#Hprep".
+      iAssert (⌜wrst = wrs⌝)%I as %->.
+      { iClear "Hinv". iNamed "Htxn".
+        iDestruct "Hprep" as "[#Hwrsrcpt _]".
+        by iDestruct (txn_wrs_agree with "Hwrsrcpt Htxnwrs") as %?.
+      }
+      wp_apply (wp_Txn__commit_in_abort_future with "Hlnrzed Hprep [$Htxn $Htida]").
+      iIntros ([]).
+    }
+    { (* Case: Commit branch. *)
+      destruct form as [| | wrs | wrs]; [done | done | done |].
+      apply dec_stable in HQ. simpl in Hpeek.
+      subst Qr.
+      destruct HQ as [HQ Hdomwrs].
+      iMod (txnsys_inv_linearize_commit wrs Q with "Htidlb Hdbpts Htxnsys Hkeys")
+        as "(Hdbpts & Htxnsys & Hkeys & Htidc & Hwrsexcl & Hclients & #HQ & #Hlnrzs & #Hlnrzed)".
+      { apply Hdomwrs. }
+      { apply Hdomr. }
+      { apply Htidgt. }
+      { apply Hpeek. }
+      (* Choose the will-commit branch. *)
+      iMod ("HAUC" $! true (wrs ∪ rds) with "[$Hdbpts]") as "HΦ"; first done.
+      iMod "Hclose" as "_".
+      iMod ("HinvC" with "[Hts Htxnsys Hkeys Hgroups Hrgs]") as "_".
+      { iNamed "Htxnsys". iFrame "∗ # %". }
+      iClear "Hinv".
+      (* Allocate transaction local view [txnmap_ptstos τ r]. *)
+      iMod (txnmap_alloc rds) as (τ) "[Htxnmap Htxnpts]".
+      iIntros "!> Htxn".
+      iAssert (own_txn txn tid rds γ τ)%I with "[Htxn Htxnmap]" as "Htxn".
+      { do 2 iNamed "Htxn".
+        iExists _, ∅.
+        rewrite map_empty_union.
+        by iFrame "∗ # %".
+      }
+
+      (*@     cmt := body(txn)                                                    @*)
+      (*@                                                                         @*)
+      wp_apply ("Hbody" with "[$Htxn $Htxnpts]"); first done.
+      iIntros (cmt) "[Htxn Hpts]".
+
+      (*@     if !cmt {                                                           @*)
+      (*@         // This transaction has not really requested to prepare yet, so no @*)
+      (*@         // cleanup tasks are required.                                  @*)
+      (*@         txn.cancel()                                                    @*)
+      (*@         return false                                                    @*)
+      (*@     }                                                                   @*)
+      (*@                                                                         @*)
+      wp_if_destruct.
+      { wp_apply (wp_Txn__cancel_in_commit_future with "[$Htxn $Htidc $Hwrsexcl]").
+        iIntros ([]).
+      }
+
+      (*@     status := txn.prepare()                                             @*)
+      (*@                                                                         @*)
+      clear HQ.
+      iDestruct "Hpts" as (w) "([%HQ %Hdomw] & [HRc _] & Hpts)".
+      iAssert (|={⊤}=> ∃ wrst, own_txn_stable txn tid rds wrst γ τ ∗ ⌜w = wrst ∪ rds⌝)%I
+        with "[Htxn Hwrsexcl Hpts]" as "Htxn".
+      { clear p.
+        iDestruct "Htxn" as (p wrst) "Htxn". iNamed "Htxn".
+        iDestruct (txnmap_subseteq with "Htxnmap Hpts") as %Hsubseteq.
+        unshelve epose proof (subseteq_dom_eq _ _ Hsubseteq _) as Heq.
+        { clear -Hincl Hdomw. set_solver. }
+        subst w.
+        iInv "Hinv" as "> HinvO" "HinvC".
+        iNamed "HinvO".
+        iMod (txnsys_inv_preprepare with "HQ Hwrsexcl Htxnsys") as "[Htxnsys Hwrsrcpt]".
+        { apply Hvts. }
+        { apply Hvwrs. }
+        { done. }
+        iMod ("HinvC" with "[$Htxnsys $Hkeys $Hgroups $Hrgs]") as "_".
+        iFrame "∗ # %".
+        do 2 iNamed "Hwrs".
+        iFrame "∗ %".
+        iApply fupd_sep.
+        iSplitL; last done.
+        rewrite -big_sepM2_fupd.
+        iApply (big_sepM2_mono with "Hpwrsm").
+        iIntros (g r m Hr Hm) "Hm".
+        by iMod (own_map_persist with "Hm") as "Hm".
+      }
+      iMod "Htxn" as (wrst) "[Htxn %Heq]". subst w.
+      wp_apply (wp_Txn__prepare with "Htxn").
+      iIntros (status) "[Htxn Hstatus]".
+
+      (*@     if status == TXN_COMMITTED {                                        @*)
+      (*@         // A backup coordinator must have committed this transaction, so simply @*)
+      (*@         // reset the write-set here.                                    @*)
+      (*@         txn.reset()                                                     @*)
+      (*@         return true                                                     @*)
+      (*@     }                                                                   @*)
+      (*@                                                                         @*)
+      wp_if_destruct.
+      { destruct status eqn:Hstatus; [done | | done]. clear Heqb.
+        subst status.
+        iDestruct "Hstatus" as (wrsc) "#Hwrsc".
+        iNamed "Htxn".
+        (* Obtain [wrsc = wrs ∧ wrst = wrs]. *)
+        iAssert (|={⊤}=> own_cmt_tmod γ tid wrs ∗ ⌜wrsc = wrs ∧ wrst = wrs⌝)%I
+          with "[Htidc]" as "Htidc".
+        { iInv "Hinv" as "> HinvO" "HinvC".
+          iNamed "HinvO". do 2 iNamed "Htxnsys".
+          iDestruct (txn_res_lookup with "Hresm Hwrsc") as %Hwrsc.
+          iDestruct (elem_of_committed_partitioned_tids with "Hpart") as %[Hnotinwc Hnotinwa].
+          { by eauto. }
+          iDestruct (cmt_tmod_lookup with "Htidcs Htidc") as %Htidc.
+          apply Htidcs in Htidc.
+          (* Prove [resm !! tid = Some (ResCommitted wrs)]. *)
+          destruct Htidc as [Htmodcs | Hresm].
+          { by rewrite not_elem_of_dom Htmodcs in Hnotinwc. }
+          rewrite Hresm in Hwrsc. symmetry in Hwrsc. inv Hwrsc.
+          iDestruct (big_sepM_lookup with "Hvr") as "Hr"; first apply Hresm.
+          iDestruct "Hr" as "[Hrcp _]".
+          iDestruct (txn_wrs_agree with "Hrcp Htxnwrs") as %->.
+          iMod ("HinvC" with "[-Htidc]") as "_".
+          { by iFrame "∗ # %". }
+          by iFrame "∗ %".
+        }
+        iMod "Htidc" as "[Htidc %Heq]".
+        destruct Heq as [-> ->].
+        iNamed "Htxn".
+        wp_apply (wp_Txn__reset with "[$Hwrs $Hptgs]").
+        iIntros "[Hwrs Hptgs]".
+        wp_pures.
+        iApply "HΦ".
+        by iFrame "∗ # %".
+      }
+      rename Heqb into Hstatusnc.
+
+      (*@     if status == TXN_ABORTED {                                          @*)
+      (*@         // Ghost action: Abort this transaction.                        @*)
+      (*@         txn.abort()                                                     @*)
+      (*@         return false                                                    @*)
+      (*@     }                                                                   @*)
+      (*@                                                                         @*)
+      wp_if_destruct.
+      { destruct status eqn:Hstatus; [done | done |]. clear Heqb.
+        subst status. simpl.
+        wp_apply (wp_Txn__abort_in_commit_future with "Hstatus [$Htxn $Htidc]").
+        iIntros ([]).
+      }
+      rename Heqb into Hstatusna.
+
+      (*@     // Ghost action: Commit this transaction.                           @*)
+      (*@     txn.commit()                                                        @*)
+      (*@     return true                                                         @*)
+      (*@ }                                                                       @*)
+      destruct status as [| |] eqn:Hstatus; [| done | done].
+      simpl. clear Hstatus Hstatusnc Hstatusna.
+      iDestruct "Hstatus" as (wrsc) "#Hprep".
+      iAssert (⌜wrsc = wrst⌝)%I as %->.
+      { iNamed "Htxn".
+        iDestruct "Hprep" as "[Hwrsrcpt _]".
+        by iDestruct (txn_wrs_agree with "Htxnwrs Hwrsrcpt") as %?.
+      }
+      wp_apply (wp_Txn__commit with "Hlnrzed Hprep [Htxn Htidc]").
+      { iFrame "∗ #". }
+      iIntros "[Htxn %Heq]". subst wrst.
+      wp_pures.
+      iApply "HΦ".
+      by iFrame.
+    }
+  Qed.
+
+  Theorem wp_Txn__Write txn tid key value rds γ τ :
+    {{{ own_txn txn tid rds γ τ ∗ (∃ vprev, txnmap_ptsto τ key vprev) }}}
+      Txn__Write #txn #(LitString key) #(LitString value)
+    {{{ RET #(); own_txn txn tid rds γ τ ∗ txnmap_ptsto τ key (Some value) }}}.
+  Proof.
+    iIntros (Φ) "[Htxn [%v Hpt]] HΦ".
+    wp_rec.
+
+    (*@ func (txn *Txn) Write(key string, value string) {                       @*)
+    (*@     v := tulip.Value{                                                   @*)
+    (*@         Present : true,                                                 @*)
+    (*@         Content : value,                                                @*)
+    (*@     }                                                                   @*)
+    (*@     txn.setwrs(key, v)                                                  @*)
+    (*@ }                                                                       @*)
+    iNamed "Htxn".
+    wp_pures.
+    wp_apply (wp_Txn__setwrs _ _ (Some value) with "Hwrs").
+    iIntros "Hwrs".
+    wp_pures.
+    iApply "HΦ".
+    iDestruct (txnmap_lookup with "Htxnmap Hpt") as %Hlookup.
+    apply elem_of_dom_2 in Hlookup.
+    iMod (txnmap_update (Some value) with "Htxnmap Hpt") as "[Htxnmap Hpt]".
+    rewrite insert_union_l.
+    iFrame "∗ # %".
+    iPureIntro.
+    rewrite /valid_wrs dom_insert_L.
+    set_solver.
+  Qed.
+
+  Theorem wp_Txn__Delete txn tid key rds γ τ :
+    {{{ own_txn txn tid rds γ τ ∗ (∃ vprev, txnmap_ptsto τ key vprev) }}}
+      Txn__Delete #txn #(LitString key)
+    {{{ RET #(); own_txn txn tid rds γ τ ∗ txnmap_ptsto τ key None }}}.
+  Proof.
+    iIntros (Φ) "[Htxn [%v Hpt]] HΦ".
+    wp_rec.
+
+    (*@ func (txn *Txn) Delete(key string) {                                    @*)
+    (*@     v := tulip.Value{                                                   @*)
+    (*@         Present : false,                                                @*)
+    (*@     }                                                                   @*)
+    (*@     txn.setwrs(key, v)                                                  @*)
+    (*@ }                                                                       @*)
+    iNamed "Htxn".
+    wp_pures.
+    wp_apply (wp_Txn__setwrs _ _ None with "Hwrs").
+    iIntros "Hwrs".
+    wp_pures.
+    iApply "HΦ".
+    iDestruct (txnmap_lookup with "Htxnmap Hpt") as %Hlookup.
+    apply elem_of_dom_2 in Hlookup.
+    iMod (txnmap_update None with "Htxnmap Hpt") as "[Htxnmap Hpt]".
+    rewrite insert_union_l.
+    iFrame "∗ # %".
+    iPureIntro.
+    rewrite /valid_wrs dom_insert_L.
+    set_solver.
+  Qed.
+
+  Theorem wp_Txn__Read txn tid key value rds γ τ  :
+    {{{ own_txn txn tid rds γ τ ∗ txnmap_ptsto τ key value }}}
+      Txn__Read #txn #(LitString key)
+    {{{ (ok : bool), RET (dbval_to_val (if ok then value else None), #ok);
+        own_txn txn tid rds γ τ ∗ txnmap_ptsto τ key value
+    }}}.
+  Proof.
+    iIntros (Φ) "[Htxn Hpt] HΦ".
+    wp_rec.
+
+    (*@ func (txn *Txn) Read(key string) (tulip.Value, bool) {                  @*)
+    (*@     vlocal, hit := txn.getwrs(key)                                      @*)
+    (*@     if hit {                                                            @*)
+    (*@         return vlocal, true                                             @*)
+    (*@     }                                                                   @*)
+    (*@                                                                         @*)
+    iNamed "Htxn".
+    wp_apply (wp_Txn__getwrs with "Hwrs").
+    iIntros (vlocal ok) "[Hwrs %Hv]".
+    iDestruct (txnmap_lookup with "Htxnmap Hpt") as %Hvalue.
+    wp_if_destruct.
+    { (* Prove [vlocal = value]. *)
+      apply (lookup_union_Some_l _ rds) in Hv.
+      rewrite Hv in Hvalue.
+      inv Hvalue.
+      wp_pures.
+      iApply ("HΦ" $! true).
+      by iFrame "∗ # %".
+    }
+    clear Heqb ok.
+
+    (*@     gid := KeyToGroup(key)                                              @*)
+    (*@     gcoord := txn.gcoords[gid]                                          @*)
+    (*@     v, ok := gcoord.Read(txn.ts, key)                                   @*)
+    (*@                                                                         @*)
+    wp_apply wp_KeyToGroup.
+    iIntros (gid Hgid).
+    iNamed "Hgcoords".
+    wp_loadField.
+    wp_apply (wp_MapGet with "Hgcoords").
+    iIntros (gcoord ok) "[%Hget Hgcoords]".
+    destruct ok; last first.
+    { apply map_get_false in Hget as [Hget _].
+      rewrite -not_elem_of_dom Hdomgcoords -Hgid in Hget.
+      by pose proof (elem_of_key_to_group key).
+    }
+    apply map_get_true in Hget.
+    iDestruct (big_sepM_lookup with "Hgcoordsabs") as "Hgcoordabs"; first apply Hget.
+    iNamed "Htxn".
+    wp_loadField.
+    wp_apply (wp_GroupCoordinator__Read with "Hgcoordabs").
+    iIntros (v ok) "#Hread".
+    wp_pures.
+
+    (*@     if !ok {                                                            @*)
+    (*@         return tulip.Value{}, false                                     @*)
+    (*@     }                                                                   @*)
+    (*@                                                                         @*)
+    destruct ok; wp_pures; last first.
+    { iApply ("HΦ" $! false).
+      iAssert (own_txn_gcoords txn γ)%I with "[$HgcoordsP $Hgcoords]" as "Hgcoords".
+      { by iFrame "# %". }
+      by iFrame "∗ # %".
+    }
+    rewrite Htsword.
+
+    (*@     trusted_proph.ResolveRead(txn.proph, txn.ts, key)                   @*)
+    (*@                                                                         @*)
+    rewrite lookup_union_r in Hvalue; last apply Hv.
+    iDestruct (big_sepM_lookup with "Hlnrz") as "Hhistl"; first apply Hvalue.
+    do 2 wp_loadField.
+    wp_apply wp_ResolveRead; first done.
+    iInv "Hinv" as "> HinvO" "HinvC".
+    iApply ncfupd_mask_intro; first set_solver.
+    iIntros "Hmask".
+    iNamed "HinvO".
+    iDestruct (txnsys_inv_extract_future with "Htxnsys") as (future) "[Hproph Htxnsys]".
+    iFrame "Hproph".
+    iIntros "(%future' & %Hfuture & Hproph)".
+    pose proof (elem_of_key_to_group key) as Hin.
+    iDestruct (big_sepS_elem_of_acc with "Hgroups") as "[Hgroup HgroupsC]".
+    { apply Hin. }
+    iDestruct (big_sepS_elem_of_acc with "Hrgs") as "[Hrg HrgsC]".
+    { apply Hin. }
+    iDestruct (big_sepS_elem_of_acc _ _ key with "Hkeys") as "[Hkey HkeysC]".
+    { apply elem_of_dom_2 in Hvalue. set_solver. }
+    iMod (txnsys_inv_read with "Hread Hhistl Htxnsys Hgroup Hrg Hkey")
+      as "(Htxnsys & Hgroup & Hrg & Hkey & %Heq)".
+    { rewrite /valid_ts in Hvts. lia. }
+    { by rewrite Hfuture. }
+    iDestruct ("HrgsC" with "Hrg") as "Hrgs".
+    iDestruct ("HgroupsC" with "Hgroup") as "Hgroups".
+    iDestruct ("HkeysC" with "Hkey") as "Hkeys".
+    rewrite Hfuture /=.
+    iDestruct (txnsys_inv_merge_future with "Hproph Htxnsys") as "Htxnsys".
+    iMod "Hmask" as "_".
+    iMod ("HinvC" with "[$Htxnsys $Hkeys $Hgroups $Hrgs]") as "_".
+    iIntros "!> _".
+    wp_pures.
+    subst value.
+
+    (*@     return v, true                                                      @*)
+    (*@ }                                                                       @*)
+    iApply ("HΦ" $! true).
+    iAssert (own_txn_gcoords txn γ)%I with "[$HgcoordsP $Hgcoords]" as "Hgcoords".
+    { by iFrame "# %". }
+    by iFrame "∗ # %".
+  Qed.
+
+End program.
